src/QFBVSimple.v
@@ -105,7 +105,7 @@ Module Make (V : SsrOrderedType) (A : Arch).
       | bvFalse => false
       | bvTrue => true
       | bvEq w e1 e2 => eval_exp e1 s == eval_exp e2 s
-      | bvUlt w e1 e2 => true (* TODO *)
+      | bvUlt w e1 e2 => ltB (eval_exp e1 s) (eval_exp e2 s)
       | bvUle w e1 e2 => true (* TODO *)
       | bvUgt w e1 e2 => true (* TODO *)
       | bvUge w e1 e2 => true (* TODO *)
